linux/pkvm/proofs/early_alloc/generated_spec.v
@@ -8,6 +8,7 @@ Section spec.
 
   (* Inlined code. *)
 
+  Definition PAGE_SHIFT := (12).
   Definition PAGE_SIZE := (4096).
 
   Definition PAGES (n : nat) : layout :=
@@ -94,7 +95,7 @@ Section spec.
 
   (* Specifications for function [hyp_early_alloc_contig]. *)
   Definition type_of_hyp_early_alloc_contig :=
-    fn(∀ (base, given, remaining, n) : loc * Z * Z * Z; (n @ (int (u32))); (global_with_type "mem" Own (((base, given, remaining)) @ (region))) ∗ ⌜0 < n ≤ remaining⌝)
+    fn(∀ (base, given, remaining, n) : loc * Z * Z * Z; (n @ (int (u32))); (global_with_type "mem" Own (((base, given, remaining)) @ (region))) ∗ ⌜0 < n ≤ remaining⌝ ∗ ⌜n ≪ PAGE_SHIFT ≤ max_int u32⌝)
       → ∃ () : (), (&own (uninit (PAGES (Z.to_nat n)))); (global_with_type "mem" Own (((base, given + n, remaining - n)%Z) @ (region))).
 
   (* Specifications for function [hyp_early_alloc_page]. *)
