linux/pkvm/proofs/early_alloc/generated_proof_hyp_early_alloc_contig.v
@@ -1,1 +1,33 @@
-(* Let's skip that, you seem to have some faith. *)
+From refinedc.typing Require Import typing.
+From refinedc.linux.pkvm.early_alloc Require Import generated_code.
+From refinedc.linux.pkvm.early_alloc Require Import generated_spec.
+From refinedc.linux.pkvm.early_alloc Require Import instances.
+Set Default Proof Using "Type".
+
+(* Generated from [linux/pkvm/early_alloc.c]. *)
+Section proof_hyp_early_alloc_contig.
+  Context `{!typeG Σ} `{!globalG Σ}.
+
+  (* Typing proof for [hyp_early_alloc_contig]. *)
+  Lemma type_hyp_early_alloc_contig (global_mem : loc) :
+    global_locs !! "mem" = Some global_mem →
+    ⊢ typed_function (impl_hyp_early_alloc_contig global_mem) type_of_hyp_early_alloc_contig.
+  Proof.
+    Open Scope printing_sugar.
+    start_function "hyp_early_alloc_contig" ([[[base given] remaining] n]) => arg_nr_pages local_i local_ret local_p.
+    split_blocks ((
+      ∅
+    )%I : gmap label (iProp Σ)) ((
+      ∅
+    )%I : gmap label (iProp Σ)).
+    - repeat liRStep; liShow.
+      all: print_typesystem_goal "hyp_early_alloc_contig" "#0".
+    Unshelve. all: sidecond_hook; prepare_sideconditions; normalize_and_simpl_goal; try solve_goal; unsolved_sidecond_hook.
+    all: unfold PAGE_SIZE, PAGE_SHIFT in *; try solve_goal.
+    + assert (0 ≤ n ≪ 12); last by lia. by apply Z.shiftl_nonneg.
+    + transitivity max_alloc_end; last done; etransitivity; last exact H10; rewrite Z.shiftl_mul_pow2 -?Z.add_assoc => //=; apply -> Z.add_le_mono_l; lia.
+    + rewrite Z.shiftl_mul_pow2 in H18 => //. lia.
+    + rewrite Z.shiftl_mul_pow2 //=. lia.
+    all: print_sidecondition_goal "hyp_early_alloc_contig".
+  Qed.
+End proof_hyp_early_alloc_contig.
