linux/pkvm/proofs/early_alloc/instances.v
@@ -1,4 +1,5 @@
 From refinedc.typing Require Import typing.
+From refinedc.linux.pkvm.early_alloc Require Import generated_spec.
 Set Default Proof Using "Type".
 
 Remove Hints find_in_context_type_val_P_own_singleton_inst : typeclass_instances.
@@ -29,6 +30,26 @@ Section instances.
   Global Instance simplify_hyp_place_combine_offset_inst l β n ty:
     SimplifyHypPlace (l.1, l.2 + n) β ty (Some 0%N) :=
     λ T, i2p (simplify_hyp_place_combine_offset l β n ty T).
+
+  Lemma simplify_hyp_place_shift_loc_assoc l β n1 n2 ty T:
+    ((l +ₗ (n1 + n2)) ◁ₗ{β} ty -∗ T) -∗ simplify_hyp ((l +ₗ n1 +ₗ n2) ◁ₗ{β} ty) T.
+  Proof. by rewrite shift_loc_assoc. Qed.
+  Global Instance simplify_hyp_place_shift_loc_assoc_inst l β n1 n2 ty:
+    SimplifyHypPlace (l +ₗ n1 +ₗ n2) β ty (Some 0%N) :=
+    λ T, i2p (simplify_hyp_place_shift_loc_assoc l β n1 n2 ty T).
+
+  Lemma simplify_hyp_place_PAGES_stuff l β n1 n2 ty T:
+    ⌜0 ≤ n2⌝ ∗((l +ₗ ((n1 + n2) * PAGE_SIZE)) ◁ₗ{β} ty -∗ T) -∗
+    simplify_hyp ((l +ₗ (n1 * PAGE_SIZE + ly_size (PAGES (Z.to_nat n2)))) ◁ₗ{β} ty) T.
+  Proof.
+    iIntros "[% HT]".
+    assert (Z.of_nat (ly_size (PAGES (Z.to_nat n2))) = n2 * PAGE_SIZE) as ->.
+    { rewrite /PAGES /ly_size /ly_with_align /= Nat2Z.inj_mul Z2Nat.id //. }
+    rewrite Z.mul_add_distr_r. done.
+  Qed.
+  Global Instance simplify_hyp_place_PAGES_stuff_inst l β n1 n2 ty:
+    SimplifyHypPlace (l +ₗ (n1 * PAGE_SIZE + ly_size (PAGES (Z.to_nat n2)))) β ty (Some 0%N) :=
+    λ T, i2p (simplify_hyp_place_PAGES_stuff l β n1 n2 ty T).
 
   Lemma simplify_goal_place_combine_offset l β n ty T:
     T ((l +ₗ n) ◁ₗ{β} ty) -∗ simplify_goal ((l.1, l.2 + n) ◁ₗ{β} ty) T.
@@ -71,6 +92,50 @@ Section instances.
   Global Instance intro_persistent_loc_in_bounds l n:
     IntroPersistent (loc_in_bounds l n) (loc_in_bounds l n).
   Proof. constructor. by iIntros "#H !>". Qed.
+
+  Lemma simplify_hyp_loc_in_bounds_ptr_in_range l (n : nat) T:
+    (⌜min_alloc_start ≤ l.2 ∧ l.2 + n ≤ max_alloc_end⌝ -∗ loc_in_bounds l n -∗ T) -∗
+    simplify_hyp (loc_in_bounds l n) T.
+  Proof.
+    iIntros "HT Hlib".
+    iDestruct (loc_in_bounds_ptr_in_range with "Hlib") as %?.
+    by iApply "HT".
+  Qed.
+  (* FIXME limit the application in a cleaner way. *)
+  Global Instance simplify_hyp_loc_in_bounds_ptr_in_range_inst l n `{!TCUnless (FastDone (min_alloc_start ≤ l.2))}:
+    SimplifyHyp (loc_in_bounds l n) (Some 0%N) :=
+    λ T, i2p (simplify_hyp_loc_in_bounds_ptr_in_range l n T).
+
+  Lemma subsume_uninit_uninit_PAGES p n1 n2 (T : iProp Σ):
+    ⌜n2 ≤ n1⌝%nat ∗ ((p +ₗ ly_size (PAGES n2)) ◁ₗ uninit (PAGES (n1 - n2)) -∗ T) -∗
+    subsume (p ◁ₗ uninit (PAGES n1))%I (p ◁ₗ uninit (PAGES n2))%I T.
+  Proof.
+    iIntros "[% HT] Hp". rewrite /uninit /ty_own /=.
+    iDestruct "Hp" as (v Hly1 Hly2) "Hp".
+    rewrite -(take_drop (ly_size (PAGES n2)) v).
+    rewrite /heap_mapsto_own_state heap_mapsto_app.
+    iDestruct "Hp" as "[Hp Hp+n2]".
+    iSplitL "Hp".
+    - iExists _. iFrame. iSplit; iPureIntro.
+      + rewrite /has_layout_val in Hly1.
+        rewrite /has_layout_val take_length Hly1.
+        rewrite /PAGES /PAGE_SIZE /ly_with_align /ly_size /=.
+        rewrite min_l //=. lia.
+      + move: Hly2. by rewrite /has_layout_loc /aligned_to /PAGES /ly_with_align /ly_align.
+    - iApply ("HT" with "[Hp+n2]").
+      rewrite /has_layout_val in Hly1.
+      rewrite take_length min_l; last first.
+      { rewrite Hly1 /PAGES /PAGE_SIZE /ly_with_align /ly_size /=. lia. }
+      iExists _. iFrame. iSplit; iPureIntro.
+      + rewrite /has_layout_val drop_length Hly1.
+        rewrite /PAGES /PAGE_SIZE /ly_with_align /ly_size /=. lia.
+      + move: Hly2. rewrite /has_layout_loc /aligned_to /ly_align /ly_size /=.
+        rewrite /PAGE_SIZE. move => Hly2. apply Z.divide_add_r => //.
+        rewrite Nat2Z.inj_mul. apply Z.divide_mul_r. rewrite Z2Nat.id => //.
+  Qed.
+  Global Instance subsume_uninit_uninit_PAGES_inst p n1 n2:
+    Subsume (p ◁ₗ uninit (PAGES n1))%I (p ◁ₗ uninit (PAGES n2))%I :=
+    λ T, i2p (subsume_uninit_uninit_PAGES p n1 n2 T).
 End instances.
 
 Typeclasses Opaque FindLocInBounds.
